cfrontend/SimplLocalsproof.v
@@ -222,12 +222,12 @@ Proof.
   induction 1; intros tyl F; inv F; constructor; eauto. eapply val_casted_inject; eauto.
 Qed.
 
-Inductive val_casted_list: list val -> typelist -> Prop :=
+Inductive val_casted_list: list val -> list type -> Prop :=
   | vcl_nil:
-      val_casted_list nil Tnil
+      val_casted_list nil nil
   | vcl_cons: forall v1 vl ty1 tyl,
       val_casted v1 ty1 -> val_casted_list vl tyl ->
-      val_casted_list (v1 :: vl) (Tcons  ty1 tyl).
+      val_casted_list (v1 :: vl) (ty1 :: tyl).
 
 Lemma val_casted_list_params:
   forall params vl,
@@ -2328,7 +2328,5 @@ Local Transparent Linker_fundef.
   destruct f1; monadInv H3; destruct f2; monadInv H4; try discriminate.
   destruct e; inv H2. exists (Internal x); split; auto. simpl; rewrite EQ; auto.
   destruct e; inv H2. exists (Internal x); split; auto. simpl; rewrite EQ; auto.
-  destruct (external_function_eq e e0 && typelist_eq t t1 &&
-            type_eq t0 t2 && calling_convention_eq c c0); inv H2.
-  econstructor; split; eauto. 
+  destruct andb; inv H2. econstructor; split; eauto. 
 Qed.
